theories/rust_typing/automation/loops.v
@@ -1,0 +1,273 @@
+Require Import Stdlib.Strings.String.
+From iris.proofmode Require Import coq_tactics reduction string_ident.
+From refinedrust Require Export type.
+From lithium Require Export all.
+From lithium Require Import hooks.
+From refinedrust.automation Require Import ident_to_string lookup_definition.
+From refinedrust Require Import programs.
+From refinedrust Require Import options.
+
+(** * Loopy stuff *)
+(* using our own list type here in order to be able to put iProp's in it (universe troubles) *)
+#[universes(polymorphic)]
+Inductive poly_list (T : Type) : Type :=
+  | PolyNil
+  | PolyCons (x : T) (l : poly_list T).
+Arguments PolyNil {_}.
+Arguments PolyCons {_}.
+
+#[universes(polymorphic)]
+Inductive poly_option (T : Type) : Type :=
+  | PolyNone
+  | PolySome (x : T).
+Arguments PolyNone {_}.
+Arguments PolySome {_}.
+
+(* Wrapper to store predicates of arbitrary arity. *)
+Definition wrap_inv {T} (x : T) := existT (P := id) _ x.
+(* Type of loop invariants:
+   - list of variables the invariant is over
+   - list of variables whose type is preserved
+   - list of uninit variables
+   - a predicate on the refinements,
+   - a predicate on the lifetime contexts
+   - optionally, the iterator variable, for which we pass the refinement into the invariant
+*)
+Definition bb_inv_t := (list loc * list loc * list loc * sigT (@id Type) * sigT (@id Type) * option loc)%type.
+(* Type of the loop invariant map we keep in the context *)
+Definition bb_inv_map_t := poly_list (var_name * bb_inv_t)%type.
+
+(* In [Prop] and sealed so it does not get discarded as a trivial assertion by Lithium when introducing *)
+Definition bb_inv_map_marker_def (M : bb_inv_map_t) := True.
+Definition bb_inv_map_marker_aux M : seal (bb_inv_map_marker_def M). Proof. by eexists. Qed.
+Definition bb_inv_map_marker M := (bb_inv_map_marker_aux M).(unseal).
+Definition bb_inv_map_marker_unfold M : bb_inv_map_marker M = bb_inv_map_marker_def M := (bb_inv_map_marker_aux M).(seal_eq).
+
+Lemma pose_bb_inv (M : bb_inv_map_t) :
+  bb_inv_map_marker M.
+Proof.
+  rewrite bb_inv_map_marker_unfold. done.
+Qed.
+
+(** Given a [runtime_function] [rfn], get the list of stack locations as a [constr]. *)
+Ltac gather_locals rfn :=
+  match rfn with
+  | Build_runtime_function ?fn ?l =>
+    eval simpl in (map fst l)
+  end.
+
+(** Find the invariant for basic block [loop_bb] in the invariant map [loop_inv_map].
+  Returns a uconstr option with the result. *)
+Ltac find_bb_inv loop_inv_map loop_bb :=
+  match loop_inv_map with
+  | PolyCons (loop_bb, ?inv) _ =>
+    constr:(PolySome inv)
+  | PolyCons (_, _) ?loop_inv_map2 =>
+    find_bb_inv loop_inv_map2 loop_bb
+  | PolyNil =>
+    constr:(@PolyNone bb_inv_t)
+  end.
+
+(** Find the type assignment for the location [loc] in the [env : env], and return it as a [constr]. *)
+Ltac find_type_assign_in_env loc env :=
+  lazymatch env with
+  | Enil => fail 10 "find_type_assign_in_env: no " loc " in env"
+  | Esnoc ?env2 _ (loc ◁ₗ[?π, ?b] ?r @ ?lt)%I =>
+      constr:((loc ◁ₗ[π, b] r @ lt)%I)
+  | Esnoc ?env2 _ _ => find_type_assign_in_env loc env2
+  end.
+
+(** Making strings from numbers *)
+Definition digit_to_ascii (n : nat) : ascii :=
+  match n with
+  | 0 => Ascii false false false false true true false false
+  | 1 => Ascii true false false false true true false false
+  | 2 => Ascii false true false false true true false false
+  | 3 => Ascii true true false false true true false false
+  | 4 => Ascii false false true false true true false false
+  | 5 => Ascii true false true false true true false false
+  | 6 => Ascii false true true false true true false false
+  | 7 => Ascii true true true false true true false false
+  | 8 => Ascii false false false true true true false false
+  | 9 => Ascii true false false true true true false false
+  | _ => Ascii false false false false true true false false
+  end.
+Definition nat_to_string (n : nat) : string.
+Proof.
+  refine (String.rev _).
+  refine (lt_wf_rec n (λ _, string) _).
+  intros m rec.
+  refine (match m as m' return m = m' → _ with
+          | 0 | 1 | 2 | 3 | 4 | 5 | 6 | 7 | 8 | 9  => λ _, String (digit_to_ascii m) EmptyString
+          | _ => λ Heq, _
+          end eq_refl).
+  refine (String (digit_to_ascii (m `mod` 10)) (rec (m `div` 10) _)).
+  abstract(apply Nat.div_lt; lia).
+Defined.
+
+(** Generates [count] successive fresh identifiers as Coq strings with prefix [prefix].
+  Poses the result as a hypothesis [out]. *)
+(* TODO: potentially take a list of suffix strings, so that we can we also get the variable names for the refinements, e.g. x, y? *)
+Ltac get_idents_rec' prefix count acc out :=
+  match count with
+  | 0%nat =>
+      set (out := acc)
+  | (S ?n)%nat =>
+      (* need to prefix with some symbol because just a number is not a valid ident *)
+      let count_str := eval cbv in (append "_" (nat_to_string n)) in
+      string_to_ident_cps count_str ltac:(fun count_ident =>
+      (* make a fresh identifier *)
+      let Hident := fresh prefix count_ident in
+      (* convert to string so we can store it *)
+      let Hident_str := constr:(ident_to_string! Hident) in
+      let acc := constr:(Hident_str :: acc) in
+      get_idents_rec' prefix constr:(n) constr:(acc) out)
+  end.
+Ltac get_idents_rec prefix count res :=
+  get_idents_rec' ident:(prefix) constr:(count) constr:(@nil string) ident:(res)
+.
+
+(** Finds the type assignments for the locations [local_locs] in the spatial context [spatial_env],
+  and abstracts their refinements to existentials [x_1, ..., x_n] whose names get picked from the list [ex_names : list string].
+  It needs to hold that [length ex_names ≥ length local_locs = n].
+  [base_app] is the name of a context item which will be specialized with the existentially abstracted refinements, to result in a fully applied term [base_app_specialized = base_app x_1 ... x_n] of type [iProp].
+  [base] is a term of type [iProp].
+
+  The tactic instantiates the current goal with the proposition claiming ownership of the locals, [base_app_specialized], and [base], with the existentials quantified in the term.
+
+  The implementation of this is currently quite hacky, mainly to work around Ltac's bad support for working with open terms. *)
+Ltac build_local_sepconj local_locs spatial_env ex_names base base_app :=
+  lazymatch local_locs with
+  | nil =>
+      exact ((base ∗ base_app)%I)
+  | cons ?local ?local_locs2 =>
+      let own_prop := find_type_assign_in_env local spatial_env in
+
+      (* get the name for this *)
+      lazymatch ex_names with
+      | nil => fail 10 "not enough names provided"
+      | ?name :: ?ex_names2 =>
+        string_to_ident_cps name ltac:(fun ident =>
+
+        (* create the type with existentially abstracted refinement *)
+        let abstracted_prop :=
+          lazymatch own_prop with
+          | (?loc ◁ₗ[?π, ?b] ?r @ ?lt)%I =>
+              (* crucial: we specialize a hypothesis _below_ the binder here in order to work around Ltac's restrictions for working with open terms *)
+              constr:((∃ ident, loc ◁ₗ[π, b] ident @ lt ∗
+                ltac:(specialize (base_app ident); build_local_sepconj local_locs2 spatial_env ex_names2 base base_app))%I)
+          end
+        in
+        exact (abstracted_prop))
+    end
+  end.
+
+Ltac get_Σ :=
+  let tgs := constr:(_ : typeGS _) in
+  match type of tgs with
+  | typeGS ?Σ => Σ
+  end.
+Ltac get_π :=
+  match goal with
+  | π : thread_id |- _ => π
+  end.
+
+(** Composes the loop invariant from the invariant [Inv : bb_inv_t] (a constr),
+  the runtime function [FN : runtime_function], the current Iris environment [env : env],
+  and the current contexts [current_E : elctx], [current_L : llctx],
+  and calls [cont Inv opt_var], where [Inv] is the invariant and [opt_var] is the optional iterator variable. *)
+Ltac compute_loop_invariant FN Inv envs current_E current_L cont :=
+  (* find Σ *)
+  let Σ := get_Σ in
+  (* get spatial env *)
+  let envs := eval hnf in envs in
+  let spatial_env :=
+    match envs with
+    | Envs _ ?spatial _ => spatial
+    | _ => fail 10 "infer_loop_invariant: could not determine spatial env"
+    end
+  in
+
+  (* extract the invariants *)
+  let inv_locals :=
+    match Inv with
+    | (?inv_locals, _, _, _, _, _) => constr:(inv_locals)
+    end in
+  let preserved_locals :=
+    match Inv with
+    | (_, ?pres_locals, _, _, _, _) => constr:(pres_locals)
+    end in
+  let functional_inv := match Inv with
+                       | (_, _, _, wrap_inv ?inv, _, _) => uconstr:(inv)
+                       end
+  in
+  let llctx_inv := match Inv with
+                   | (_, _, _, _, wrap_inv ?inv, _) => uconstr:(inv)
+                   end
+  in
+  let iterator_var := match Inv with
+                   | (_, _, _, _, _, ?var) => uconstr:(var)
+                   end
+  in
+
+  (* generate names for the existentially abstracted refinements *)
+  let num_locs := eval cbv in (length inv_locals) in
+  let names_ident := fresh "tmp" in
+  get_idents_rec ident:(r) constr:(num_locs) ident:(names_ident);
+  let names := eval cbv in names_ident in
+  clear names_ident;
+
+  let Hinv := fresh "Hinv" in
+
+  (* optionally apply to the refinement of the iterator variable *)
+  let iterator_var := constr:(iterator_var) in
+  match iterator_var with
+  | Some ?var =>
+      (*let own_prop := find_type_assign_in_env var spatial_env in*)
+      (*lazymatch own_prop with*)
+      (*| (?loc ◁ₗ[?π, ?b] ?r @ ?lt)%I =>*)
+          (*specialize (Ha r)*)
+      (*end*)
+    pose (Hinv :=
+      λ (iter_init_state : _) (E : elctx) (L : llctx),
+      ltac:(
+        (* specialize the lifetime ctx invariant *)
+        let HEL := fresh "Hel" in
+        pose (HEL := (E = current_E ∧ L = current_L));
+
+        (* pose the loop invariant as a local hypothesis so we can specialize it while building the term *)
+        let Ha := fresh "Hinv" in
+        pose (Ha := functional_inv);
+
+        specialize (Ha iter_init_state);
+
+        build_local_sepconj inv_locals spatial_env names constr:(((True ∗ ⌜HEL⌝)%I: iProp Σ)) Ha
+    ));
+    (* get rid of all the lets we introduced *)
+    simpl in Hinv;
+    let Inv := eval unfold Hinv in Hinv in
+    clear Hinv;
+    cont Inv iterator_var
+
+  | None => 
+    pose (Hinv :=
+      λ (E : elctx) (L : llctx),
+      ltac:(
+        (* specialize the lifetime ctx invariant *)
+        let HEL := fresh "Hel" in
+        pose (HEL := (E = current_E ∧ L = current_L));
+
+        (* pose the loop invariant as a local hypothesis so we can specialize it while building the term *)
+        let Ha := fresh "Hinv" in
+        pose (Ha := functional_inv);
+
+        build_local_sepconj inv_locals spatial_env names constr:(((True ∗ ⌜HEL⌝)%I: iProp Σ)) Ha
+    ));
+    (* get rid of all the lets we introduced *)
+    simpl in Hinv;
+    let Inv := eval unfold Hinv in Hinv in
+    clear Hinv;
+    cont Inv (@None nat)
+  end
+
+.
